wasm-proofs/Wasm-Proof/make_coupon.thy
@@ -1,0 +1,165 @@
+theory make_coupon
+  imports self_coupon storage_coupon
+begin
+
+datatype request =
+  Blob | Self
+
+fun request_to_nat :: "request \<Rightarrow> nat" where
+  "request_to_nat Blob = 0"
+| "request_to_nat Self = 1"
+
+fun request_to_func_idx :: "request \<Rightarrow> nat" where
+  "request_to_func_idx Blob = func_make_blob_coupon_idx"
+| "request_to_func_idx Self = func_make_self_coupon_idx"
+
+fun make_coupon :: "request \<Rightarrow> handle list \<Rightarrow> handle \<Rightarrow> handle \<Rightarrow> handle option" where
+  "make_coupon Blob coupons l r = make_blob_coupon_raw coupons l r"
+| "make_coupon Self coupons l r = make_self_coupon_raw coupons l r"
+
+lemma make_coupon_blob_some:
+  assumes "make_coupon Blob coupons l r = Some res"
+  shows "make_blob_coupon_raw coupons l r = Some res"
+  using assms by auto
+
+lemma make_coupon_blob_none:
+  assumes "make_coupon Blob coupons l r = None"
+  shows "make_blob_coupon_raw coupons l r = None"
+  using assms by auto
+
+lemma make_coupon_self_some:
+  assumes "make_coupon Self coupons l r = Some res"
+  shows "make_self_coupon_raw coupons l r = Some res"
+  using assms by auto
+
+lemma make_coupon_self_none:
+  assumes "make_coupon Blob coupons l r = None"
+  shows "make_blob_coupon_raw coupons l r = None"
+  using assms by auto
+
+lemma make_coupon_prologue:
+  "run_invoke_v 
+         (n + 10)
+         (Suc depth)
+         (init\<lparr> tabs := (tabs init)[tab_coupons_idx := ((T_tab \<lparr> l_min = 0, l_max = None\<rparr> T_ext_ref), (map (\<lambda>c. (ConstRefExtern (to_externref c))) coupons))] \<rparr>,
+         [(V_num (ConstInt32 (I32.int_of_nat (request_to_nat request)))),
+          (V_ref (ConstRefExtern (to_externref l))),
+          (V_ref (ConstRefExtern (to_externref r)))],
+         func_make_coupon_idx) = (case run_iter n
+          (Config depth
+            (init\<lparr> tabs := (tabs init)[tab_coupons_idx := ((T_tab \<lparr> l_min = 0, l_max = None\<rparr> T_ext_ref), (map (\<lambda>c. (ConstRefExtern (to_externref c))) coupons))] \<rparr>)
+            (Frame_context
+              (Redex
+                [V_ref (ConstRefExtern (to_externref r)),
+                 V_ref (ConstRefExtern (to_externref l))]
+                [Invoke (request_to_func_idx request)] [])
+              [Label_context [] [] (Suc 0) [],
+               Label_context [] [] (Suc 0) []]
+              (Suc 0)
+              \<lparr>f_locs =
+                 [V_num (ConstInt32 (I32.int_of_nat (request_to_nat request))),
+                  V_ref (ConstRefExtern (to_externref l)),
+                  V_ref (ConstRefExtern (to_externref r))],
+               f_inst = exp_inst \<rparr>)
+            [Frame_context (Redex [] [] []) [] 0 empty_frame]) of
+    (Config d s fc fcs, res) \<Rightarrow> (s, res))"  
+proof -
+  have 1: "n + 10 = (Suc (Suc (Suc (Suc (Suc (Suc (Suc (Suc (Suc (Suc n))))))))))" by auto
+  show ?thesis
+  by (cases "request", auto simp add: I32.int_of_nat_def init_def tab_coupons_idx_def func_make_coupon_idx_def n_zeros_def app_f_v_s_local_get_def app_s_f_v_s_table_size_def stab_ind_def app_v_s_relop_def app_relop_def app_relop_i_def app_relop_i_v_def int_lt_u_i32_def I32.int_lt_u_def int_of_nat_i32.rep_eq I32.rep_abs app_v_s_if_def wasm_bool_def zero_i32_def int_eq_i32.abs_eq I32.int_eq_def tb_tf_def app_s_f_v_s_call_indirect_def tab_cl_ind_def nat_of_int_i32.abs_eq stypes_def cl_type_def func_make_blob_coupon_idx_def func_make_self_coupon_idx_def 1)
+qed
+
+lemma make_coupon_epilog:
+"run_iter (n + 4)
+    (Config depth s
+      (Frame_context (Redex [V_ref (ConstRefExtern (to_externref (create_eq_coupon l r)))] [] [])  
+      [Label_context [] [] (Suc 0) [], Label_context [] [] (Suc 0) []] 
+      (Suc 0) f)
+    [Frame_context (Redex [] [] []) [] 0 empty_frame]) 
+  = 
+    ((Config (Suc depth) s
+    (Frame_context (Redex [V_ref (ConstRefExtern (to_externref (create_eq_coupon l r)))] [] []) [] 0 empty_frame) [])
+    , RValue [V_ref (ConstRefExtern (to_externref (create_eq_coupon l r)))])"
+proof -
+  have 1: "4 = (Suc (Suc (Suc (Suc 0))))" by auto
+  show ?thesis by (simp add: Let_def 1)
+qed
+
+lemma make_coupon_some:
+  assumes "make_coupon request coupons l r = Some res"
+  shows "\<exists>fuel depth. run_invoke_v
+         fuel
+         depth
+         (init\<lparr> tabs := (tabs init)[tab_coupons_idx := ((T_tab \<lparr> l_min = 0, l_max = None\<rparr> T_ext_ref), (map (\<lambda>c. (ConstRefExtern (to_externref c))) coupons))] \<rparr>,
+         [(V_num (ConstInt32 (I32.int_of_nat (request_to_nat request)))),
+          (V_ref (ConstRefExtern (to_externref l))),
+          (V_ref (ConstRefExtern (to_externref r)))],
+         func_make_coupon_idx)
+         = (init\<lparr> tabs := (tabs init)[tab_coupons_idx := ((T_tab \<lparr> l_min = 0, l_max = None\<rparr> T_ext_ref), (map (\<lambda>c. (ConstRefExtern (to_externref c))) coupons))] \<rparr>, RValue [V_ref (ConstRefExtern (to_externref (create_eq_coupon l r)))])"
+proof (cases "request")
+  case Blob
+  show ?thesis
+    using make_coupon_prologue[of 35 1 coupons "Blob"]
+          make_blob_coupon_raw_run_iter[of coupons l r res 4 0 "[]"] assms
+          make_coupon_epilog[of 0 1] Blob
+    by (intro exI[where x=45]  exI[where x = "Suc (Suc 0)"]) auto
+next
+  case Self
+  show ?thesis
+    using make_coupon_prologue[of 18 1 coupons "Self"]
+          make_self_coupon_raw_run_iter[of coupons l r res 4 0 "[]"] assms
+          make_coupon_epilog[of 0 1] Self
+    by (intro exI[where x=28]  exI[where x = "Suc (Suc 0)"]) auto
+qed
+
+lemma make_coupon_none:
+  assumes "make_coupon request coupons l r = None"
+  shows "\<exists>fuel depth cfg msg. run_invoke_v
+         fuel
+         depth
+         (init\<lparr> tabs := (tabs init)[tab_coupons_idx := ((T_tab \<lparr> l_min = 0, l_max = None\<rparr> T_ext_ref), (map (\<lambda>c. (ConstRefExtern (to_externref c))) coupons))] \<rparr>,
+         [(V_num (ConstInt32 (I32.int_of_nat (request_to_nat request)))),
+          (V_ref (ConstRefExtern (to_externref l))),
+          (V_ref (ConstRefExtern (to_externref r)))],
+         func_make_coupon_idx)
+         = (cfg, RTrap msg)"
+proof -
+  have "\<exists>msg cfg. run_iter (fuel50 0)
+          (Config 
+           (Suc 1)
+           (init\<lparr> tabs := (tabs init)[tab_coupons_idx := ((T_tab \<lparr> l_min = 0, l_max = None\<rparr> T_ext_ref), (map (\<lambda>c. (ConstRefExtern (to_externref c))) coupons))] \<rparr>)
+           (Frame_context 
+              (Redex ((V_ref (ConstRefExtern (to_externref r))) #
+                      (V_ref (ConstRefExtern (to_externref l))) #
+                      [])
+                     [Invoke (request_to_func_idx request)]
+                     [])
+              [Label_context [] [] (Suc 0) [],
+               Label_context [] [] (Suc 0) []]
+              (Suc 0)
+              \<lparr>f_locs =
+                 [V_num (ConstInt32 (I32.int_of_nat (request_to_nat request))),
+                  V_ref (ConstRefExtern (to_externref l)),
+                  V_ref (ConstRefExtern (to_externref r))],
+               f_inst = exp_inst \<rparr>)
+            [Frame_context (Redex [] [] []) [] 0 empty_frame])
+        = (cfg, RTrap msg)"
+    using make_blob_coupon_raw_run_invoke_none make_self_coupon_raw_run_invoke_none assms
+    by (cases "request") auto
+
+  then have "\<exists>msg cfg. (run_invoke_v
+         ((fuel50 0) + 10)
+         (Suc (Suc 1))
+         (init\<lparr> tabs := (tabs init)[tab_coupons_idx := ((T_tab \<lparr> l_min = 0, l_max = None\<rparr> T_ext_ref), (map (\<lambda>c. (ConstRefExtern (to_externref c))) coupons))] \<rparr>,
+         [(V_num (ConstInt32 (I32.int_of_nat (request_to_nat request)))),
+          (V_ref (ConstRefExtern (to_externref l))),
+          (V_ref (ConstRefExtern (to_externref r)))],
+         func_make_coupon_idx))
+         = (case (cfg, RTrap msg) of (Config d s fc fcs, res) \<Rightarrow> (s, res))"
+    by (simp only: make_coupon_prologue) metis
+
+  then show ?thesis
+    by (metis (mono_tags, lifting) case_prod_conv config.case config.exhaust)
+qed
+
+end
