wasm-proofs/Wasm-Proof/self_coupon.thy
@@ -1,0 +1,81 @@
+theory self_coupon
+  imports Wasm_Proof_Playground
+begin
+
+fun make_self_coupon_raw :: "handle list \<Rightarrow> handle \<Rightarrow> handle \<Rightarrow> handle option" where
+"make_self_coupon_raw xs l r = 
+ (if (is_equal l r) then 
+    Some (create_eq_coupon l r) 
+  else 
+    None)"
+
+lemma ms_some:
+  assumes "make_self_coupon_raw coupons l r = Some res"
+  shows "is_equal l r \<and> res = (create_eq_coupon l r)"
+  by (metis assms make_self_coupon_raw.simps option.distinct(1) option.sel)
+
+lemma make_self_coupon_raw_run_iter:
+  assumes "make_self_coupon_raw coupons l r = Some res"
+  shows "run_iter  
+  (Suc (Suc (Suc (Suc (Suc (Suc (Suc (Suc (Suc (Suc (Suc (Suc (Suc (Suc n))))))))))))))
+  (Config 
+   (Suc n')
+   (init\<lparr> tabs := (tabs init)[tab_coupons_idx := ((T_tab \<lparr> l_min = 0, l_max = None\<rparr> T_ext_ref), (map (\<lambda>c. (ConstRefExtern (to_externref c))) coupons))] \<rparr>)
+   (Frame_context 
+      (Redex ((V_ref (ConstRefExtern (to_externref r))) #
+              (V_ref (ConstRefExtern (to_externref l))) #
+              rest_vs)
+             [Invoke func_make_self_coupon_idx]
+             b_es)
+    lc f \<lparr>f_locs = locs, f_inst = exp_inst\<rparr>) fcs)
+  =
+   run_iter n
+          (Config 
+           (Suc n')
+           (init\<lparr> tabs := (tabs init)[tab_coupons_idx := ((T_tab \<lparr> l_min = 0, l_max = None\<rparr> T_ext_ref), (map (\<lambda>c. (ConstRefExtern (to_externref c))) coupons))] \<rparr>)
+            (Frame_context (Redex (V_ref (ConstRefExtern (to_externref (create_eq_coupon l r))) # rest_vs) [] b_es) lc f  \<lparr>f_locs = locs, f_inst = exp_inst\<rparr>) fcs)"
+proof -
+  have 1: "is_equal l r" using ms_some[OF assms] by blast
+  have 2: "res = create_eq_coupon l r" using ms_some[OF assms] by blast
+
+  let ?state = " (init\<lparr> tabs := (tabs init)[tab_coupons_idx := ((T_tab \<lparr> l_min = 0, l_max = None\<rparr> T_ext_ref), (map (\<lambda>c. (ConstRefExtern (to_externref c))) coupons))] \<rparr> )"
+
+  show ?thesis
+    using fixpoint_is_equal_correct_externref[of "to_externref l" "to_externref r" ?state] 1
+    fixpoint_create_eq_coupon_impl[of ?state "to_externref l" "to_externref r"]
+    by (auto split: cl.splits simp del: split_n.simps simp add: init_def func_make_self_coupon_idx_def app_f_call_def sfunc_ind_def n_zeros_def split_n_0 split_n_1 split_n_2 app_f_v_s_local_get_def 2 typeof_def typeof_ref_def typeof_num_def tab_coupons_idx_def app_v_s_if_def se tb_tf_def)
+qed
+
+lemma ms_none:
+  assumes "make_self_coupon_raw coupons l r = None"
+  shows "\<not> is_equal l r"
+  using assms by force
+
+lemma make_self_coupon_raw_run_invoke_none:
+  assumes "make_self_coupon_raw coupons l r = None"
+  shows "\<exists>msg cfg.
+         run_iter (fuel50 n)
+         (Config
+          (Suc n')
+           (init\<lparr> tabs := (tabs init)[tab_coupons_idx := ((T_tab \<lparr> l_min = 0, l_max = None\<rparr> T_ext_ref), (map (\<lambda>c. (ConstRefExtern (to_externref c))) coupons))] \<rparr>)
+           (Frame_context 
+              (Redex ((V_ref (ConstRefExtern (to_externref r))) #
+                      (V_ref (ConstRefExtern (to_externref l))) #
+                      rest_vs)
+                     [Invoke func_make_self_coupon_idx]
+                     b_es)
+            lc f \<lparr>f_locs = locs, f_inst = exp_inst\<rparr>) fcs)
+        = (cfg, RTrap msg)"
+proof -
+  let ?state = "(init\<lparr> tabs := (tabs init)[tab_coupons_idx := ((T_tab \<lparr> l_min = 0, l_max = None\<rparr> T_ext_ref), (map (\<lambda>c. (ConstRefExtern (to_externref c))) coupons))] \<rparr> )"
+
+  have 1: "\<not>is_equal l r"
+    using ms_none[OF assms] .
+
+  show ?thesis
+    using fixpoint_is_equal_correct_externref_neq[of "to_externref l" "to_externref r" ?state] 1    
+    by (auto split: cl.splits simp del: split_n.simps simp add:  init_def func_make_self_coupon_idx_def n_zeros_def bitzero_def tab_coupons_idx_def app_s_f_v_s_table_get_def stab_ind_def load_tabs1_def
+    app_f_v_s_local_set_def app_f_v_s_local_get_def app_f_call_def sfunc_ind_def typeof_def typeof_num_def  se tb_tf_def typeof_ref_def app_v_s_binop_def app_binop_def app_binop_i_v_def app_binop_i_def split_n_0 split_n_1 split_n_2 app_v_s_if_def sf)
+qed
+
+end
